@prefix rdfs: <http://www.w3.org/2000/01/rdf-schema#> .
@prefix owl: <http://www.w3.org/2002/07/owl#> .
@prefix rdf: <http://www.w3.org/1999/02/22-rdf-syntax-ns#> .
@prefix xml: <http://www.w3.org/XML/1998/namespace> .
@prefix xsd: <http://www.w3.org/2001/XMLSchema#> .
@prefix sp: <http://spinrdf.org/sp#> .
@prefix spin: <http://spinrdf.org/spin#> .
@prefix spl: <http://spinrdf.org/spl#> .
@prefix skos: <http://www.w3.org/2004/02/skos/core#>.

# content standards
@prefix qb: <http://purl.org/linked-data/cube#> .
@prefix dcterms: <http://purl.org/dc/terms/> .


@prefix lid: <http://id.sirf.net/def/schema/lid/> .

@prefix void: <http://rdfs.org/ns/void#> .

# domain 
@prefix qb4st: <http://resources.opengeospatial.org/def/ontology/qb4st/> .
@prefix prof: <http://resources.opengeospatial.org/def/ontology/prof/> .

# Makes the set of Profiles and QB components into VoiD datasets and binds the API to them - in conjunction with the basic lid_alternates_spin rules for all datasets.
  
qb4st:ComponentRegister rdfs:subClassOf lid:lidset, skos:ConceptScheme;
   rdfs:label "The register of instances of QB Component sub types"@en ;
   rdfs:comment "Declaring the set of registered sub-types of a QB component as subclass of void:Dataset allows the attachment of metadata about the state of the register, and binds to relevant convenience APIs to access deep traversals of the inherited properties of such definitions. "@en ;
   rdfs:subClassOf [
        a owl:Restriction ;
        owl:onProperty void:feature ;
        owl:someValuesFrom prof:QbComponentInheritedView ;
     ]  ;
     . 

prof:ProfileRegister rdfs:subClassOf lid:lidset ;
    rdfs:subClassOf [
        a owl:Restriction ;
        owl:onProperty void:feature ;
        owl:someValuesFrom prof:ProfileInheritedView ;
     ]  ;
	rdfs:subClassOf [
        a owl:Restriction ;
        owl:onProperty void:feature ;
        owl:someValuesFrom prof:ProfileMinimalView ;
     ]  ;
     .


	 
prof:ProfileInheritedView a lid:LDAViewer ;
    rdfs:label "Profile encapsulated view";
    rdfs:comment "Self contained ontology view of profile with all inherited constraints";
    lid:viewName    "profile" ;
	lid:featurescope "item" ;
#    rdfs:seeAlso <http://www.w3.org/Protocols/rfc2616/rfc2616-sec14.html#>;
    .

	 
prof:ProfileMinimalView a lid:LDAViewer ;
    rdfs:label "Profile minimal view";
    rdfs:comment "The minimal view of a profile, with only inherited references";
    lid:viewName    "profile_raw" ;
	lid:featurescope "item" ;
#    rdfs:seeAlso <http://www.w3.org/Protocols/rfc2616/rfc2616-sec14.html#>;
    .

	 
prof:ProfileOWLlView a lid:LDAViewer ;
    rdfs:label "Profile minimal OWL view";
    rdfs:comment "OWL view of profile, with transitive imports";
    lid:viewName    "profile_owl" ;
    lid:featurescope "item" ;
#    rdfs:seeAlso <http://www.w3.org/Protocols/rfc2616/rfc2616-sec14.html#>;
    .
	
prof:QbComponentInheritedView  a lid:LDAViewer ;
    rdfs:label "RDF Datacube component encapsulated view";
    rdfs:comment "Self contained ontology view of a QB component (dimension or measure) with all inherited constraints";
    lid:viewName    "qb" ;
    lid:featurescope "item" ;
#    rdfs:seeAlso <http://www.w3.org/Protocols/rfc2616/rfc2616-sec14.html#>;
    .
