@prefix rdfs: <http://www.w3.org/2000/01/rdf-schema#> .
@prefix owl: <http://www.w3.org/2002/07/owl#> .
@prefix rdf: <http://www.w3.org/1999/02/22-rdf-syntax-ns#> .
@prefix xml: <http://www.w3.org/XML/1998/namespace> .
@prefix xsd: <http://www.w3.org/2001/XMLSchema#> .
@prefix sp: <http://spinrdf.org/sp#> .
@prefix spin: <http://spinrdf.org/spin#> .
@prefix spl: <http://spinrdf.org/spl#> .

# content standards
@prefix qb: <http://purl.org/linked-data/cube#> .
@prefix dcterms: <http://purl.org/dc/terms/> .

@prefix lid: <http://id.sirf.net/def/schema/lid/> .

# domain 
@prefix qb4st: <http://resources.opengeospatial.org/def/ontology/qb4st/> .
@prefix prof: <http://resources.opengeospatial.org/def/ontology/prof/> .

# Classes

<http://resources.opengeospatial.org/def/ontology/prof> a lid:lidset;
	rdfs:label "Root register for all profiles in this domain"@en;
.


prof:Profile a rdfs:Class;
	rdfs:label "An interoperability profile, defining aspects of conformant datasets." ;
	
	# spin rule to trigger RDFS entailment - Profiles are an RDFS class, datasets maybe described as instances of such profiles
	spin:rule [ 
	     a sp:Construct ;
	     rdfs:label "Makes each Profile a RDFS Class"@en;
	     rdfs:comment "spin rule to trigger RDFS entailment - Profiles are an RDFS class, datasets maybe described as instances of such profiles"@en ;
	     sp:text """
		     PREFIX rdfs: <http://www.w3.org/2000/01/rdf-schema#>
			 PREFIX prof: <http://resources.opengeospatial.org/def/ontology/prof/>
		     CONSTRUCT {
		    	?A a rdfs:Class .
				}
			 WHERE {
			    ?A a prof:Profile .
			    }
			""" ;
	    ]  ;
	
		spin:rule [ 
	     a sp:Construct ;
	     rdfs:label "Generates a VoiD dataset for the namespace, so that inherited API bindings can be exposed"@en;
	     rdfs:comment "enforces subClass for inherited models"@en ;
	     sp:text """
		     PREFIX rdfs: <http://www.w3.org/2000/01/rdf-schema#>
			 PREFIX prof: <http://resources.opengeospatial.org/def/ontology/prof/>
			 PREFIX qb: <http://purl.org/linked-data/cube#>
			 PREFIX skos: <http://www.w3.org/2004/02/skos/core#>
		        CONSTRUCT {
					?base a prof:ProfileRegister  .
					?base rdfs:label ?basestr .
					?base rdfs:comment "Profile register for the subdomain" .
				}
			 WHERE {
			    ?this a prof:Profile
				BIND ( replace( str(?this), "(#|/)[^#/]*$", "" ) as ?basestr  )
 				BIND ( IRI(?basestr) as ?base ) 
			}
			""" ;
	    ]  ;
	    
    	# spin rule to trigger RDFS entailment - Profiles are an RDFS class, datasets maybe described as instances of such profiles
	spin:rule [ 
	     a sp:Construct ;
	     rdfs:label "Makes each profile a subclass of inherited class"@en;
	     rdfs:comment "enforces subClass for inherited models"@en ;
	     sp:text """
		     PREFIX rdfs: <http://www.w3.org/2000/01/rdf-schema#>
			 PREFIX prof: <http://resources.opengeospatial.org/def/ontology/prof/>
		     CONSTRUCT {
		    	?B rdfs:subClassOf ?A .
				}
			 WHERE {
			    ?A a prof:Profile .
			    ?B a prof:Profile .
			    ?B skos:broader ?A .
			    }
			""" ;
	    ]  ;
	    
 	# rule to create a grandparent (implementsTransitive association - adds transitive semantics to the rdfs:subClass
	spin:rule [ 
	     	a sp:Construct ;
	     rdfs:comment "rule to create a grandparent (implementsTransitive association - adds transitive semantics to rdfs:subClass"@en ;
	     sp:text """
		     PREFIX rdfs: <http://www.w3.org/2000/01/rdf-schema#>
			 PREFIX prof: <http://resources.opengeospatial.org/def/ontology/prof/>
		     CONSTRUCT {
			    ?B skos:broaderTransitive ?A .
			    ?A skos:narrowerTransitive ?B .
				}
			 WHERE {
			    ?A a prof:Profile .
			    ?B a prof:Profile .
			    ?B skos:broader+ ?A .
			    }
			 """ ;
		    ]  ;
	spin:rule [ 
    	a sp:Construct ;
       	rdfs:comment "Assert that child profile also contains dimension bindings from parent (handling overidden bindings)."@en ;
	    sp:text """
			PREFIX rdfs: <http://www.w3.org/2000/01/rdf-schema#>
			PREFIX prof: <http://resources.opengeospatial.org/def/ontology/prof/>
			CONSTRUCT {
		    	?B prof:dimBinding ?dimA
			}
			WHERE {
			    ?A a prof:Profile .
			    ?B a prof:Profile .
			    ?B rdfs:subClassOf ?A .
			    ?A prof:dimBinding ?dimA .
			    FILTER NOT EXISTS {
			        ?B prof:dimBinding ?dimB .
			        ?dimB prof:overrides ?dimA .
			    }
			} """ ; 
	] ;
	spin:rule [ 
    	a sp:Construct ;
       	rdfs:comment "Assert that child profile also contains measure bindings from parent (handling overidden bindings)."@en ;
	    sp:text """
			PREFIX rdfs: <http://www.w3.org/2000/01/rdf-schema#>
			PREFIX prof: <http://resources.opengeospatial.org/def/ontology/prof/>
			CONSTRUCT {
		    	?B prof:measureBinding ?dimA
			}
			WHERE {
			    ?A a prof:Profile .
			    ?B a prof:Profile .
			    ?B rdfs:subClassOf ?A .
			    ?A prof:measureBinding ?dimA .
			    FILTER NOT EXISTS {
			        ?B prof:measureBinding ?dimB .
			        ?dimB prof:overrides ?dimA .
			    }
			} """ ; 
	] ;
.

prof:DimensionBinding a rdfs:Class;
	rdfs:subClassOf qb:ComponentSpecification ;
	rdfs:label "Dimension Binding"@en;
	rdfs:comment "Specifies a profile must have the dimension, and allows attributes to narrow the scope of the referenced qb:DimensionProperty. Equivalent to a qb:ComponentSpecification, "@en;
	spin:rule [ 
    	a sp:Construct ;
       	rdfs:comment "Identify where a measure binding is overriding an inherited binding requirement - because it binds to a subclass of a required component"@en ;
	    sp:text """
			PREFIX rdfs: <http://www.w3.org/2000/01/rdf-schema#>
			PREFIX prof: <http://resources.opengeospatial.org/def/ontology/prof/>
			PREFIX qb: <http://purl.org/linked-data/cube#>
			CONSTRUCT {
		    	?dimB prof:overrides ?dimA
			}
			WHERE {
			    ?dimA a prof:DimensionBinding .
			    ?dimB a prof:DimensionBinding FILTER ( ?dimA != ?dimB ) .
			    ?dimA qb:dimension ?A .
			    ?dimB qb:dimension ?B .
			    ?B rdfs:subClassOf+ ?A FILTER ( ?A != ?B ) .
			} """ ; 
	] ;
.

prof:MeasureBinding a rdfs:Class;
	rdfs:subClassOf qb:ComponentSpecification ;
	rdfs:label "Measure Binding"@en;
	rdfs:comment "Specifies a profile must have the measure, and allows attributes to narrow the scope of the referenced qb:MeasureProperty"@en;
	spin:rule [ 
    	a sp:Construct ;
       	rdfs:comment "Identify where a measure binding is overriding an inherited binding requirement - because it binds to a subclass of a required component"@en ;
	    sp:text """
			PREFIX rdfs: <http://www.w3.org/2000/01/rdf-schema#>
			PREFIX prof: <http://resources.opengeospatial.org/def/ontology/prof/>
			PREFIX qb: <http://purl.org/linked-data/cube#>
			CONSTRUCT {
		    	?dimB prof:overrides ?dimA
			}
			WHERE {
			    ?dimA a prof:MeasureBinding .
			    ?dimB a prof:MeasureBinding .
			    ?dimA qb:measure ?A .
			    ?dimB qb:measure ?B .
			    ?B rdfs:subClassOf ?A .
			} """ ; 
	] ;
	.



prof:dimBinding a rdfs:Property;
	rdfs:subPropertyOf qb:component ;
	rdfs:range prof:DimemsionBinding;
	
.


