@prefix rdfs: <http://www.w3.org/2000/01/rdf-schema#> .
@prefix owl: <http://www.w3.org/2002/07/owl#> .
@prefix rdf: <http://www.w3.org/1999/02/22-rdf-syntax-ns#> .
@prefix xml: <http://www.w3.org/XML/1998/namespace> .
@prefix xsd: <http://www.w3.org/2001/XMLSchema#> .
@prefix sp: <http://spinrdf.org/sp#> .
@prefix spin: <http://spinrdf.org/spin#> .
@prefix spl: <http://spinrdf.org/spl#> .

# content standards
@prefix qb: <http://purl.org/linked-data/cube#> .
@prefix dcterms: <http://purl.org/dc/terms/> .

@prefix lid: <http://id.sirf.net/def/schema/lid/> .

# domain 
@prefix qb4st: <http://resources.opengeospatial.org/def/ontology/qb4st/> .


# Classes
qb4st:ComponentRegister a rdfs:Class;
	rdfs:label "A Class declaration for sets of QB components"@en;
	rdfs:comment "To be extended to bind metadata and API behaviour to deployed set, as required. This is sufficient for entailment rules to make each namespace in which components are defined into a sub-register"@en;
	.

# Properties
qb4st:implements a rdfs:Property;
	rdfs:label "inherits constraints from the related object";
	# meta:rangeIncludes qb:ComponentProperty
	# meta:domainIncludes qb:ComponentProperty
	rdfs:comment "Could be a subProperty of rfds:subClassOf - an inheritance mechanism that triggers overrides of ranges etc"@en ;
.

qb4st:implementsTransitive a rdfs:Property;
	rdfs:label "indirect inheritance . ";
	# meta:rangeIncludes qb:ComponentProperty
	# meta:domainIncludes qb:ComponentProperty
	rdfs:comment "Convenience handled by entailment, listing all sources of inherited properties"@en ;
.

qb4st:implementedBy a rdfs:Property;
	rdfs:label "link to implementing sub-classes";
	# meta:rangeIncludes qb:ComponentProperty
	# meta:domainIncludes qb:ComponentProperty
	rdfs:comment "Convenience links, generated by entailment"@en ;
.




